\section{Temporary}
Let $A$ be a finite set, $x_1$ be the word of $A$ 
that it's subsetc construction is as the followings:
\begin{equation}\begin{split}
	x_1 &= a_1\rhd x_2 \\
	x_2 &= a_2\rhd x_3 \\
	&\vdots \\
\end{split}\end{equation}
, where $a_1,a_2,\dots\in A$  and $x_1,x_2,\dots\in FA$.
We shall consider the word $y_1=\bakko{A^*}x_1$.
The subset construction of $y_1$ is as the followings:
\begin{equation}\begin{split}
	y_1 &= \bakko{A^*}x_1 \\
		&= a_1\rhd x_2 + A\rhd y_1 \\
		&= a_1\rhd (x_2+y_1) + a_1^c\rhd y_1 \\
		&= a_1\rhd y_2 + a_1^c\rhd y_1 \\
	y_2 &= x_2 + y_1 \\
		&= a_2\rhd x_3 + a_1\rhd y_2 + a_1^c\rhd y_1 \\
		&= \begin{cases}
			a_1=a_2 \implies & a_2\rhd (x_3+y_2) + a_2^c\rhd y_1 \\
			a_1\not=a_2 \implies & a_2\rhd (x_3+y_1) + a_1\rhd y_2 + a_1^c\wedge a_2^c\rhd y_1 \\
			\end{cases} \\
		&= \begin{cases}
			a_1=a_2 \implies & a_2\rhd (x_3+y_2) + a_2^c\rhd y_1 \\
			a_1\not=a_2 \implies & a_2\rhd (x_3+y_1) + a_2^c\wedge(a_1\rhd y_2 + a_1^c\rhd y_1) \\
			\end{cases} \\
		&= \begin{cases}
			a_1=a_2 \implies & a_2\rhd y_3 + a_2^c\rhd y_1 \\
			a_1\not=a_2 \implies & a_2\rhd y_3 + a_2^c\wedge y_1 \\
			\end{cases} \\
	y_3 &= \begin{cases}
			a_1=a_2 \implies & x_3+y_2 \\
			a_1\not=a_2 \implies & x_3+y_1 \\
			\end{cases} \\
		&= \begin{cases}
			a_1=a_2 \implies & a_3\rhd x_4 + a_2\rhd y_3 + a_2^c\rhd y_1 \\
			a_1\not=a_2 \implies & a_3\rhd x_4 + a_1\rhd y_2 + a_1^c\rhd y_1 \\
			\end{cases} \\
		&= \begin{cases}
			a_1=a_2\wedge a_2=a_3 \implies & a_3\rhd (x_4 + y_3) + a_3^c\rhd y_1 \\
			a_1=a_2\wedge a_2\not=a_3 \implies & a_3\rhd (x_4 + y_1) + a_3^c\wedge(a_2\rhd y_3 + a_2^c\rhd y_1) \\
			a_1\not=a_2\wedge a_1=a_3 \implies & a_3\rhd (x_4 + y_2) + a_3^c\rhd y_1 \\
			a_1\not=a_2\wedge a_1\not=a_3 \implies & a_3\rhd (x_4 + y_1) + a_3^c\wedge(a_1\rhd y_2 + a_1^c\rhd y_1) \\
			\end{cases} \\
		&= \begin{cases}
			a_1=a_2\wedge a_2=a_3 \implies & a_3\rhd y_4 + a_3^c\rhd y_1 \\
			a_1=a_2\wedge a_2\not=a_3 \implies & a_3\rhd y_4 + a_3^c\wedge y_2 \\
			a_1\not=a_2\wedge a_1=a_3 \implies & a_3\rhd y_4 + a_3^c\rhd y_1 \\
			a_1\not=a_2\wedge a_1\not=a_3 \implies & a_3\rhd y_4 + a_3^c\wedge y_1 \\
			\end{cases} \\
	y_4 &= \begin{cases}
			a_1=a_2\wedge a_2=a_3 \implies & x_4+y_3 \\
			a_1\not=a_2\wedge a_1=a_3 \implies & x_4+y_2 \\
			a_1\not=a_3 \implies & x_4+y_1 \\
			\end{cases} \\
\end{split}\end{equation}
induction for $2\le m$
\begin{equation}\begin{split}
	\tau m &\in \set{1,2,\dots,m-1} \\
	y_m &= x_m + y_{\tau m} \\
		&= \begin{cases}
			a_m\rhd y_{m+1} + a_m^c\rhd y_1 & \text{iff }a_m=a_{\tau m} \\
			a_m\rhd y_{m+1} + a_m^c\wedge y_{\tau m} & \text{else} \\
			\end{cases} \\
\end{split}\end{equation}
, then
\begin{equation}\begin{split}
	y_m &= x_m + y_{\tau m} \\
		&= \begin{cases}
			a_{\tau m}=a_{\tau^2 m}\implies & a_m\rhd x_{m+1} + a_{\tau m}\rhd y_{\tau m+1} + a_{\tau m}^c\rhd y_{1} \\
			a_{\tau m}\not=a_{\tau^2 m}\implies & a_m\rhd x_{m+1} + a_{\tau m}\rhd y_{\tau m+1} + a_{\tau m}^c\wedge y_{\tau^2 m} \\
			\end{cases} \\
		&= \begin{cases}
			a_{\tau m}=a_{\tau^2 m}\wedge a_m=a_{\tau m}\implies & a_m\rhd (x_{m+1} + y_{\tau m+1}) + a_m^c\rhd y_{1} \\
			a_{\tau m}=a_{\tau^2 m}\wedge a_m\not=a_{\tau m}\implies & a_m\rhd (x_{m+1} + y_{1}) + a_m^c\wedge y_{\tau m} \\
			a_{\tau m}\not=a_{\tau^2 m}\wedge a_m=a_{\tau m}\implies & a_m\rhd (x_{m+1} + y_{\tau m+1}) + a_m^c\rhd y_{\tau^2 m} \\
			a_{\tau m}=a_{\tau^2 m}\wedge a_m\not=a_{\tau m}\implies & a_m\rhd (x_{m+1} + y_{\tau^2 m}) + a_m^c\wedge y_{\tau m} \\
			\end{cases} \\
		&\Downarrow \\
	\tau(m+1) &= \begin{cases}
		a_m=a_{\tau m}\implies & \tau m + 1 \\
		a_{\tau m}=a_{\tau^2 m}\wedge a_m\not=a_{\tau m}\implies & 1 \\
		a_{\tau m}\not=a_{\tau^2 m}\wedge a_m\not=a_{\tau m}\implies & \tau^2 m \\
		\end{cases} \\
\end{split}\end{equation}

